ExistentialRules/Triggers/RTrigger.lean
@@ -29,5 +29,14 @@ namespace RTrigger
 /-- Two `RTrigger`s are equivalent if the underlying `PreTrigger`s are. -/
 abbrev equiv {rs : RuleSet sig} (trg1 trg2 : RTrigger obs rs) : Prop := trg1.val.equiv trg2.val
 
+/-- Lifting the definition from `PreTrigger`. -/
+abbrev extend_with_groundTermMapping {rs : RuleSet sig} (trg : RTrigger obs rs) (h : GroundTermMapping sig) : RTrigger obs rs :=
+  ⟨trg.val.extend_with_groundTermMapping h, trg.property⟩
+
+/-- We can boil `extend_with_groundTermMapping` down to the `PreTrigger` version again. -/
+@[simp, grind =]
+theorem val_extend_with_groundTermMapping {rs : RuleSet sig} {trg : RTrigger obs rs} {h : GroundTermMapping sig} :
+  (trg.extend_with_groundTermMapping h).val = PreTrigger.extend_with_groundTermMapping trg.val h := rfl
+
 end RTrigger
 
